----------------------------------------------
-- Proof of consistency using a glued model --
----------------------------------------------

module Consistency.Glueing where

open import Lib
open import CLT
open import Norm

private
  variable
    a b c : Ty

-- a "submodel" (called glued model) equipped with a proof
-- that quot is homomorphic on the reduction relation _âŸ¶*_
-- Note: this submodel acts as *necessary* technical device
-- to prove consistency (see below)
Gl : âŸ¦ a âŸ§ â†’ Set
Gl {Nat}   n = âŠ¤
Gl {a â‡’ b} f = âˆ€ (x : âŸ¦ a âŸ§) â†’ Gl x
  â†’ (quot f âˆ™ quot x âŸ¶* quot (f âˆ™' x))
  Ã— Gl (f âˆ™' x)
Gl {a + b} (injâ‚ x) = Gl x
Gl {a + b} (injâ‚‚ y) = Gl y
Gl {ğŸ™}     tt       = âŠ¤

-- application for glued values
appg : {f : âŸ¦ a â‡’ b âŸ§} {x : âŸ¦ a âŸ§}
  â†’ Gl f â†’ Gl x
  â†’ Gl (f âˆ™' x)
appg fg xg = Ï€â‚‚ (fg _ xg)

-- primitive recursion for glued values
recg : {x : âŸ¦ a âŸ§} {f :  âŸ¦ Nat â‡’ a â‡’ a âŸ§ } {n : âŸ¦ Nat âŸ§}
  â†’ Gl x â†’ Gl f â†’ Gl n â†’ Gl (rec' x f n)
recg {n = zero}  xg fg ng = xg
recg {n = suc n} xg fg ng =
  appg (appg fg ng) (recg {n = n} xg fg ng)

caseg : {f : âŸ¦ a â‡’ c âŸ§} â†’ {g : âŸ¦ b â‡’ c âŸ§} â†’ {s : âŸ¦ a + b âŸ§}
  â†’ Gl f â†’ Gl g â†’ Gl s â†’ Gl (case' f g s)
caseg {s = injâ‚ x} fg gg sg = appg fg sg
caseg {s = injâ‚‚ y} fg gg sg = appg gg sg

-- homomorphism properties of quot

hom-app : {f : âŸ¦ a â‡’ b âŸ§} {x : âŸ¦ a âŸ§}
  â†’ Gl f â†’ Gl x
  â†’ quot f âˆ™ quot x âŸ¶* quot (f âˆ™' x)
hom-app fg xg = Ï€â‚ (fg _ xg)

hom-rec : {x : âŸ¦ a âŸ§} {f : âŸ¦ Nat â‡’ a â‡’ a âŸ§ } {n : âŸ¦ Nat âŸ§}
    â†’ Gl x â†’ Gl f â†’ Gl n
    â†’ quot (eval Rec âˆ™' x âˆ™' f) âˆ™ quot n
    âŸ¶* quot (rec' x f n)
hom-rec {n = zero}  xg fg ng = lift rec0
hom-rec {x = x} {f} {n = suc n} xg fg ng =
      recs â—… trans
        (app* (hom-app fg ng) (hom-rec {n = n} xg fg _))
        (hom-app (appg fg _) (recg {n = n} xg fg _))

hom-case : {f : âŸ¦ a â‡’ c âŸ§ } {g : âŸ¦ b â‡’ c âŸ§} {s : âŸ¦ a + b âŸ§}
    â†’ Gl f â†’ Gl g â†’ Gl s
    â†’ quot (eval Case âˆ™' f âˆ™' g) âˆ™ quot s
    âŸ¶* quot (case' f g s)
hom-case {s = injâ‚ x} fg gg sg = trans (lift redl) (hom-app fg sg)
hom-case {s = injâ‚‚ y} fg gg sg = trans (lift redr) (hom-app gg sg)

open import Function

-- interpretation of terms in the glued model
-- Note: main challenge here is to provide a proof
-- object that quot is a homomorphism in each case
gl : (t : Tm a) â†’  Gl (eval t)
gl K x xg    = refl , Î» x _ â†’ (lift redk) , xg
gl Zero      = tt
gl Succ      = Î» x _ â†’ refl , tt
gl (t âˆ™ u) = Ï€â‚‚ (gl t _ (gl u))
gl S g gg    = refl , Î» f fg â†’
  refl , Î» x xg â†’
       reds â—… trans
         (app* (hom-app gg xg) (hom-app fg xg))
         (hom-app (appg gg xg) (appg fg xg))
      , appg (appg gg xg) (appg fg xg)
gl Rec x xg   = refl , (Î» f fg â†’
  refl , Î» n ng â†’
    hom-rec {n = n} xg fg ng , (recg {n = n} xg fg ng))
gl Inl x xg = refl , xg
gl Inr x xg = refl , xg
gl (Case) f fg = refl , Î» g gg â†’
  refl , Î» s sg â†’ hom-case {s = s} fg gg sg , caseg {s = s} fg gg sg
gl Init  x xg = âŠ¥-elim x
gl Unit = tt

-- normalization is consistent with reduction (_âŸ¶*_)
-- or, loosely speaking, `norm` transforms by reduction
consistent-red* : (t : Tm a) â†’ t âŸ¶* em (norm t)
consistent-red* K = refl
consistent-red* S = refl
consistent-red* Zero = refl
consistent-red* Succ = refl
consistent-red* Rec = refl
consistent-red* (t âˆ™ u) = trans
  (app* (consistent-red* t) (consistent-red* u))
  (hom-app (gl t) (gl u))
consistent-red* Inl  = refl
consistent-red* Inr  = refl
consistent-red* Case = refl
consistent-red* Unit = refl
consistent-red* Init = refl

-- normalization is consistent with conversion
consistent : (t : Tm a) â†’ t â‰ˆ em (norm t)
consistent t = âŸ¶*â†’â‰ˆ (consistent-red* t)
