--------------------------------------------------
-- Proof of consistency using logical relations --
--------------------------------------------------

-- An alternative to the glued submodel construction

module Consistency.LR where

open import Lib
open import CLT
open import Norm
open import Soundness

private
  variable
    a b c : Ty

-- logical relations for proving consistency
R : Tm a â†’ âŸ¦ a âŸ§ â†’ Set
R {Nat}   n m = n âŸ¶* quot m
R {a â‡’ b} t f = t âŸ¶* quot f
  Ã— ({u : Tm a} {u' : âŸ¦ a âŸ§}
  â†’ R u u'
  â†’ R (t âˆ™ u) (f âˆ™' u'))
R {a + b} t (injâ‚ x)
  = âˆƒ (Î» u â†’ R u x Ã— t âŸ¶* Inl âˆ™ u)
R {a + b} t (injâ‚‚ y)
  = âˆƒ (Î» u â†’ R u y Ã— t âŸ¶* Inr âˆ™ u)
R {ğŸ™}     t v = t âŸ¶* quot v

-- R implies reduction by _âŸ¶*_ (by reifying the value on right)
-- (the whole purpose of R!)
R-reduces : {t : Tm a} {x : âŸ¦ a âŸ§}
  â†’ R t x
  â†’ t âŸ¶* quot x
R-reduces {Nat}   p       = p
R-reduces {a â‡’ b} (p , _) = p
R-reduces {a + b} {x = injâ‚ _} (_ , q , r) = trans r (app* refl (R-reduces q))
R-reduces {a + b} {x = injâ‚‚ _} (_ , q , r) = trans r (app* refl (R-reduces q))
R-reduces {ğŸ™} p = p

-- Note: Due to `R-reduces`, we may simply
-- say "t reduces to v" for `R t v`
-- instead of "t is related by R to v"

-- invariance lemma
R-resp-â‰ˆ : {f g : Tm a} {x : âŸ¦ a âŸ§}
  â†’ g âŸ¶* f
  â†’ R f x
  â†’ R g x
R-resp-â‰ˆ {Nat} gâ‰ˆf rfx
  = trans gâ‰ˆf rfx
R-resp-â‰ˆ {_ â‡’ _} p   (q , r)
  = trans p q , Î» y â†’ R-resp-â‰ˆ (app* p refl) (r y)
R-resp-â‰ˆ {_ + _} {x = injâ‚ _} p (u , q , r)
  = u , q , trans p r
R-resp-â‰ˆ {_ + _} {x = injâ‚‚ _} p (u , q , r)
  = u , q , trans p r
R-resp-â‰ˆ {ğŸ™} p q
  = trans p q

-- syntactic application reduces to semantic application
R-app : {t : Tm (a â‡’ b)} {f : âŸ¦ a â‡’ b âŸ§}
  {u : Tm a} {x : âŸ¦ a âŸ§}
  â†’ R t f
  â†’ R u x
  â†’ R (t âˆ™ u) (f âˆ™' x)
R-app (p , q) r = q r

-- syntactic recursion reduces to semantic recursion
R-rec : {e : Tm a} {v : âŸ¦ a âŸ§}
  {t : Tm (Nat â‡’ a â‡’ a)} {f : âŸ¦ Nat â‡’ a â‡’ a âŸ§}
  {n : Tm Nat} {m : âŸ¦ Nat âŸ§}
  â†’ R e v
  â†’ R t f
  â†’ R n m
  â†’ R (Rec âˆ™ e âˆ™ t  âˆ™ n) (rec' v f m)
R-rec {m = zero} p q r
  = R-resp-â‰ˆ (trans (app* refl r) (lift rec0)) p
R-rec {m = suc m} p q r
  = R-resp-â‰ˆ
      (trans (app* refl r) (lift recs))
      (R-app (R-app q refl) (R-rec {m = m} p q refl))

R-case : {t : Tm (a â‡’ c)} {f : âŸ¦ a â‡’ c âŸ§}
  {u : Tm (b â‡’ c)} {g : âŸ¦ b â‡’ c âŸ§}
  {s : Tm (a + b)} {v : âŸ¦ a + b âŸ§}
  â†’ R t f
  â†’ R u g
  â†’ R s v
  â†’ R (Case âˆ™ t âˆ™ u âˆ™ s) (case' f g v)
R-case {v = injâ‚ x} p _ (t' , q , r)
  = R-resp-â‰ˆ
      (trans (app* refl r) (lift redl))
      (R-app p q)
R-case {v = injâ‚‚ y} _ p (t' , q , r)
  = R-resp-â‰ˆ
      (trans (app* refl r) (lift redr))
      (R-app p q)

-- fundamental theorem of R
-- i.e., a term reduces to its interpretation
fund : (t : Tm a) â†’ R t (eval t)
fund K = refl , Î» p â†’
  (app* refl (R-reduces p)) , Î» q â†’
    R-resp-â‰ˆ (lift redk) p
fund S = refl , Î» p â†’
  app* refl (R-reduces p) , Î» q â†’
    (app* (app* refl (R-reduces p)) (R-reduces q)) , Î» r â†’
      R-resp-â‰ˆ (lift reds) (R-app (R-app p r) (R-app q r))
fund Zero = refl
fund Succ
  = refl , Î» p â†’ (app* refl p)
fund Rec
  = refl , Î» p â†’
    (app* refl (R-reduces p)) , Î» q â†’
      (app* (app* refl (R-reduces p)) (R-reduces q)) , Î» {_} {n} r â†’
        R-rec {m = n} p q r
fund (t âˆ™ u) = R-app (fund t) (fund u)
fund Inl = refl , Î» p â†’ _ , p , refl
fund Inr = refl , Î» p â†’ _ , p , refl
fund Case = refl , Î» p â†’
  app* refl (R-reduces p) , Î» q â†’
    (app* (app* refl (R-reduces p)) (R-reduces q)) , Î» r â†’
      R-case p q r
fund Unit = refl
fund Init = refl , Î» {_} {bot} x â†’ âŠ¥-elim bot

-- proof of consistency by R

consistent-red* : (t : Tm a) â†’ t âŸ¶* em (norm t)
consistent-red* t = R-reduces (fund t)

consistent : (t : Tm a) â†’ t â‰ˆ em (norm t)
consistent t = âŸ¶*â†’â‰ˆ (consistent-red* t)
